First stab at renaming local constants

ST/Logic.v
@@ -294,44 +294,87 @@ Fixpoint list_evars_term (t : Term) (l : list nat) : list nat :=
 match t with
 | Var _ => l
 | EConst n => insert n l
-| Fun f args => Vector.fold_left (fun l' => fun (arg : Term) => insert_merge l' (list_evars_term arg l'))
+| Fun f args => Vector.fold_left (fun l' => fun (arg : Term) => insert_merge (list_evars_term arg l') l')
     l args
 end.
+
+Theorem list_evars_term_sorted : forall (t : Term) (l : list nat),
+  sorted l -> sorted (list_evars_term t l).
+Proof.
+  intros.
+  induction t.
+  - assert (list_evars_term (Var v) l = l). { simpl; auto. }
+    rewrite H0. assumption.
+  - assert (list_evars_term (EConst n) l = insert n l). { simpl; auto. }
+    rewrite H0. apply insert_preserves_sorted. assumption.
+  - rename t into args.
+    assert (list_evars_term (Fun n0 args) l = Vector.fold_left (fun l' => fun (arg : Term) => insert_merge (list_evars_term arg l') l')
+    l args). { simpl; auto. }
+    rewrite H0. apply insert_merge_vector_fold_sorted2.
+    assumption.
+Qed.
 
 Global Instance EnumerateEVarsTerm : EnumerateEVars Term := {
   list_evars tm := list_evars_term tm []
 }.
 
-Hypothesis list_evers_term_sorted : forall (t : Term),
+Theorem list_evers_term_sorted : forall (t : Term),
   sorted (list_evars t).
+Proof. intros.
+  unfold list_evars; unfold EnumerateEVarsTerm.
+  assert (sorted []%list). { apply sorted_nil. }
+  apply list_evars_term_sorted.
+  assumption.
+Qed.
 
 Global Instance EnumerateEVarsPredicate : EnumerateEVars Predicate := {
 list_evars p := match p with
-| P n s args => Vector.fold_left (fun l' => fun (arg : Term) => insert_merge l' (list_evars arg)) []%list args
+| P n s args => Vector.fold_left (fun l' => fun (arg : Term) => insert_merge (list_evars arg) l') []%list args
 end
 }.
 
-Hypothesis list_evars_predicate_sorted : forall (p : Predicate),
+Theorem list_evars_predicate_sorted : forall (p : Predicate),
   sorted (list_evars p).
+Proof. intros.
+  destruct p.
+  rename t into args.
+  unfold list_evars; unfold EnumerateEVarsPredicate.
+  apply insert_merge_vector_fold_sorted2.
+  apply sorted_nil.
+Qed.
 
 Global Instance EnumerateEVarsRadix : EnumerateEVars Radix := {
 list_evars R := match R with
 | Ast => []%list
-| Mode n s args => Vector.fold_left (fun l' => fun (arg : Term) => insert_merge l' (list_evars arg)) []%list args
+| Mode n s args => Vector.fold_left (fun l' => fun (arg : Term) => insert_merge (list_evars arg) l') []%list args
 end
 }.
 
-Hypothesis list_evars_radix_sorted : forall (R : Radix),
+Theorem list_evars_radix_sorted : forall (R : Radix),
   sorted (list_evars R).
+Proof.
+  intros.
+  induction R.
+  - simpl; auto. apply sorted_nil.
+  - rename t into args.
+    unfold list_evars; unfold EnumerateEVarsRadix.
+    apply insert_merge_vector_fold_sorted2.
+    apply sorted_nil.
+Qed.
 
 Global Instance EnumerateEVarsAttribute : EnumerateEVars Attribute := {
 list_evars attr := match attr with
-| Attr n s args => Vector.fold_left (fun l' => fun (arg : Term) => insert_merge l' (list_evars arg)) []%list args
+| Attr n s args => Vector.fold_left (fun l' => fun (arg : Term) => insert_merge (list_evars arg) l') []%list args
 end
 }.
 
-Hypothesis list_evars_attribute_sorted : forall (A : Attribute),
+Theorem list_evars_attribute_sorted : forall (A : Attribute),
   sorted (list_evars A).
+Proof. intros. destruct A. rename t into args.
+  unfold list_evars; unfold EnumerateEVarsAttribute.
+  apply insert_merge_vector_fold_sorted2.
+  apply sorted_nil.
+Qed.
 
 Global Instance EnumerateEVarsAdjective : EnumerateEVars Adjective := {
 list_evars adj := match adj with
@@ -353,13 +396,19 @@ Qed.
 
 Global Instance EnumerateEVarsSoftType : EnumerateEVars SoftType := {
 list_evars T := match T with
-| (adjectives,T) => List.fold_left (fun l' => fun (adj : Adjective) => insert_merge l' (list_evars adj))
+| (adjectives,T) => List.fold_left (fun l' => fun (adj : Adjective) => insert_merge (list_evars adj) l')
  adjectives (list_evars T)
 end
 }.
 
-Hypothesis list_evars_soft_type_sorted : forall (T : SoftType),
+Theorem list_evars_soft_type_sorted : forall (T : SoftType),
   sorted (list_evars T).
+Proof. intros. destruct T.
+  assert (sorted (list_evars r)). { apply list_evars_radix_sorted. }
+  unfold list_evars; unfold EnumerateEVarsSoftType.
+  apply insert_merge_list_fold_sorted2 with (init := list_evars r).
+  assumption.
+Qed.
 
 Global Instance EnumerateEVarsJudgementType : EnumerateEVars JudgementType := {
 list_evars Judg := match Judg with
@@ -371,30 +420,61 @@ list_evars Judg := match Judg with
 end
 }.
 
-Hypothesis list_evars_judgement_type_sorted : forall (j : JudgementType),
+Theorem list_evars_judgement_type_sorted : forall (j : JudgementType),
   sorted (list_evars j).
+Proof.
+  intros. induction j.
+  - unfold list_evars; unfold EnumerateEVarsJudgementType. apply sorted_nil.
+  - unfold list_evars; unfold EnumerateEVarsJudgementType.
+    assert (sorted (list_evars s)). { apply list_evars_soft_type_sorted. }
+    apply insert_merge_sorted2. assumption.
+  - unfold list_evars; unfold EnumerateEVarsJudgementType.
+    assert (sorted (list_evars s0)). { apply list_evars_soft_type_sorted. }
+    apply insert_merge_sorted2. assumption.
+  - unfold list_evars; unfold EnumerateEVarsJudgementType.
+    assert (sorted (list_evars s)). { apply list_evars_soft_type_sorted. }
+    assumption.
+  - unfold list_evars; unfold EnumerateEVarsJudgementType.
+    assert (sorted (list_evars s)). { apply list_evars_soft_type_sorted. }
+    apply insert_merge_sorted2. assumption.
+Qed.
+
+Definition evars_local_declaration (d : Decl) :=
+  match d with
+  | (_, T) => (list_evars T)
+  end.
 
 Global Instance EnumerateEVarsLocalContext : EnumerateEVars LocalContext := {
 list_evars lc := List.fold_left (fun l' => fun (d : Decl) => 
-  match d with
-  | (_, T) => insert_merge l' (list_evars T)
-  end)
+  insert_merge (evars_local_declaration d) l')
  lc []%list
 }.
 
-Hypothesis list_evars_local_context_sorted : forall (lc : LocalContext),
+Theorem list_evars_local_context_sorted : forall (lc : LocalContext),
   sorted (list_evars lc).
+Proof. intros.
+  unfold list_evars; unfold EnumerateEVarsLocalContext.
+  apply insert_merge_list_fold_sorted. apply sorted_nil.
+Qed.
+
+Definition list_evars_gc_def (d : LocalContext * JudgementType) :=
+match d with
+  | (lc, T) => insert_merge (list_evars lc) (list_evars T)
+  end.
 
 Global Instance EnumerateEVarsGlobalContext : EnumerateEVars GlobalContext := {
 list_evars gc := List.fold_left (fun l' => fun d => 
-  match d with
-  | (lc, T) => insert_merge l' (insert_merge (list_evars lc) (list_evars T))
-  end)
+  insert_merge (list_evars_gc_def d)  l')
  gc []%list
 }.
 
-Hypothesis list_evars_global_context_sorted : forall (gc : GlobalContext),
+Theorem list_evars_global_context_sorted : forall (gc : GlobalContext),
   sorted (list_evars gc).
+Proof.
+  intros.
+  unfold list_evars; unfold EnumerateEVarsGlobalContext.
+  apply insert_merge_list_fold_sorted. apply sorted_nil.
+Qed.
 
 Global Instance EnumerateEVarsJudgement : EnumerateEVars Judgement := {
 list_evars j := match j with
@@ -402,8 +482,17 @@ list_evars j := match j with
 end
 }.
 
-Hypothesis list_evars_judgement_sorted : forall (j : Judgement),
+Theorem list_evars_judgement_sorted : forall (j : Judgement),
   sorted (list_evars j).
+Proof. intros. destruct j.
+  unfold list_evars; unfold EnumerateEVarsJudgement.
+  assert (sorted (list_evars j)). { apply list_evars_judgement_type_sorted. }
+  destruct p.
+  assert (sorted (insert_merge (list_evars l) (list_evars j))). {
+    apply insert_merge_sorted2; assumption.
+  }
+  apply insert_merge_sorted2; assumption.
+Qed.
 
 Fixpoint list_evars_formula (phi : Formula) : list nat :=
 match phi with
@@ -417,273 +506,31 @@ Global Instance EnumerateEVarsFormula : EnumerateEVars Formula := {
 list_evars := list_evars_formula
 }. 
 
-Hypothesis list_evars_formula_sorted : forall (phi : Formula),
+Theorem list_evars_formula_sorted : forall (phi : Formula),
   sorted (list_evars phi).
+Proof. intros. induction phi.
+- simpl; auto. apply sorted_nil.
+- unfold list_evars; unfold EnumerateEVarsFormula. apply list_evars_predicate_sorted.
+- unfold list_evars; unfold EnumerateEVarsFormula.
+  apply insert_merge_sorted2; assumption.
+- unfold list_evars; unfold EnumerateEVarsFormula.
+  apply insert_merge_sorted2; assumption.
+- unfold list_evars; unfold EnumerateEVarsFormula.
+  apply insert_merge_sorted2; assumption.
+- simpl; auto.
+Qed.
 
 Global Instance EnumerateEVarsFormulaList : EnumerateEVars (list Formula) := {
-list_evars Γ := (List.fold_left (fun l' => fun (phi : Formula) => insert_merge l' (list_evars phi))
+list_evars Γ := (List.fold_left (fun l' => fun (phi : Formula) => insert_merge (list_evars phi) l')
  Γ []%list)
 }. 
 
-Hypothesis list_evars_formula_list_sorted : forall (l : list Formula),
+Theorem list_evars_formula_list_sorted : forall (l : list Formula),
   sorted (list_evars l).
-
-Require Import Nat.
-Require Import Coq.Arith.PeanoNat.
-  Check Nat.eqb_eq.
-
-Lemma first_new_cons {l n} :
-  first_new n (n :: l) = first_new (S n) l.
 Proof.
-  assert(n = n). reflexivity.
-  apply Nat.eqb_eq in H as H1.
-  simpl; auto. rewrite H1. reflexivity.
+  intros. unfold list_evars; unfold EnumerateEVarsFormulaList.
+  apply insert_merge_list_fold_sorted. apply sorted_nil.
 Qed.
-
-Lemma neq_neqb : forall (n k : nat),
-  n <> k <-> Nat.eqb n k = false.
-Proof. intros. revert n.
-  induction k as [|k IHk]; intro n; destruct n; simpl; rewrite ?IHk; split; try easy.
-  - intros. assert (n <> k). red; auto. apply IHk in H0. assumption.
-  - intros. apply IHk in H. red; auto.
-Qed.
-
-Lemma first_new_distinct {l a n} :
-  a <> n -> first_new n (a :: l) = first_new n l.
-Proof. 
-  intros. 
-  apply neq_neqb in H as H1.
-  simpl; auto. rewrite H1. 
-  reflexivity.
-Qed.
-
-Lemma fresh_new_step {l n k} :
-  first_new n l = first_new n (k::l) \/ first_new (S n) l = first_new n (k::l).
-Proof.
-  assert({k = n} + {k <> n}). decide equality. destruct H.
-  - right. rewrite e. symmetry. apply first_new_cons.
-  - left. apply (@first_new_distinct l k n) in n0. symmetry; assumption.
-Qed.
-
-Lemma first_new_nondecreasing {l n} :
-  n <= first_new n l.
-Proof. generalize dependent n.
-  induction l. 
-  - simpl; auto.
-  - intros. assert ({a = n} + {a <> n}). decide equality.
-    destruct H.
-  -- rewrite e. 
-     assert (first_new n (n :: l) = first_new (S n) l).
-     apply first_new_cons. rewrite H.
-     assert (S n <= first_new (S n) l). apply (@IHl (S n)).
-     intuition.
-  -- assert(first_new n l = first_new n (a :: l)). symmetry. apply (@first_new_distinct l a n).
-     assumption. rewrite <- H.
-     apply IHl.
-Qed.  
-
-Lemma fresh_succ_nonzero {l n} :
-  0 < first_new (S n) l.
-Proof.
-  intros. generalize dependent n. induction l.
-  - simpl; auto. apply Nat.lt_0_succ.
-  - intros. destruct (@fresh_new_step l (S n) a).
-  + rewrite <- H. apply IHl.
-  + rewrite <- H. apply (IHl (S n)).
-Qed.
-
-(*
-Lemma first_new_cons_inv {l n a} :
-  a = n <-> first_new n (a :: l) = first_new (S n) l.
-Proof.
-  assert ({a = n} + {a <> n}). decide equality. destruct H.
-  - split.
-  -- rewrite e. intros. apply first_new_cons.
-  -- intros; assumption.
-  - split. contradiction. intros. inversion H.
-    assert (Nat.eqb a n  = false). { apply neq_neqb. assumption. }
-    rewrite H0 in H1.
-  split. 
-  - intros. rewrite H. apply first_new_cons.
-  - intros. inversion H.
-  assert(n = n). reflexivity.
-  apply Nat.eqb_eq in H as H1.
-  simpl; auto. rewrite H1. reflexivity.
-Qed.
-*)
-Require Import Coq.Arith.Compare.
-
-Lemma first_new_on_different_args {l m n} :
-  m <= n -> first_new m l <= first_new n l.
-Proof.
-  intros. generalize dependent m. generalize dependent n.
-  induction l.
-  - simpl; auto.
-  - intros.
-    assert ({n = a} + {n <> a}). decide equality. destruct H0.
-  + assert (first_new n (n :: l) = first_new (S n) l). apply first_new_cons.
-    assert ({m = a} + {m <> a}). decide equality. destruct H1.
-  ++ rewrite e0; rewrite <- e. reflexivity.
-  ++ (* m <> a && n = a *)
-    assert (first_new m (a :: l) = first_new m l). {
-    apply (@first_new_distinct l a m); intuition.
-    }
-    rewrite H1. 
-    assert (n <= first_new n (a :: l)). { apply first_new_nondecreasing. }
-    rewrite <- e; rewrite H0. apply IHl. intuition.
-  + (* n <> a *)
-    assert (first_new n (a :: l) = first_new n l). { apply (@first_new_distinct l a n); intuition. }
-    assert ({m = a} + {m <> a}). decide equality. destruct H1.
-  ++ (* n <> a && m = a *)
-     assert (first_new m (a :: l) = first_new (S m) l). {
-       rewrite <- e; apply first_new_cons.
-     }
-     Check le_le_S_eq.
-     assert (S m <= n \/ m = n). { apply le_le_S_eq in H. assumption. }
-     destruct H2.
- +++ (* S m <= n *)
-     rewrite H0. rewrite H1. apply IHl. intuition.
- +++ rewrite H2. reflexivity.
- ++ assert (first_new m (a :: l) = first_new m l). { apply (@first_new_distinct l a m); intuition. }
-    rewrite H1; rewrite H0. apply IHl. assumption.
-Qed.
-
-Require Import Lia.
-Require Import Coq.Lists.ListDec Decidable.
-
-Theorem first_new_sorted {l n} :
-  sorted l -> ~(In (first_new n l) l).
-Proof. intros.
-  inversion H.
-  - simpl; auto.
-  - assert({x = n} + {x <> n}). decide equality. destruct H1.
-  + rewrite e.
-    assert (first_new n [n] = first_new (S n) []). apply (@first_new_cons List.nil).
-    rewrite H1. unfold first_new. apply not_in_cons. simpl; auto.
-  + assert(first_new n [x] = first_new n []). { apply first_new_distinct. assumption. } 
-    rewrite H1. unfold first_new. apply not_in_cons. simpl; auto.
-  - admit.
-Qed.
-
-Lemma first_new_is_not_in_list {l n} :
-  ~(In (first_new n l) l).
-Proof. generalize dependent n.
-  induction l.
-  - simpl; auto.
-  - intros. assert({a = n} + {a <> n}). decide equality. destruct H.
- -- (* a = n *) 
-    assert(first_new n (a::l) = first_new (S n) l). { rewrite e. apply first_new_cons. }
-    apply not_in_cons. split.
-    + rewrite e; apply not_eq_sym; apply first_new_distinct2.
-    + rewrite H. apply IHl.
- -- (* a <> n *)
-    apply not_in_cons. split.
-    + apply first_new_distinct3.
-    + apply (first_new_distinct (l := l)) in n0 as H. rewrite H. apply IHl.
-Qed.
-
-Lemma first_new_is_new {l n} :
-  forall (x : nat), In x l -> first_new n l <> x.
-Proof.
-  induction l.
-  - simpl; auto.
-  - intros. assert ({a = n} + {a <> n}). decide equality. destruct H0.
- -- (* Case: a = n *) 
-    rewrite e.
-    assert(first_new n (n::l) = first_new (S n) l). { apply first_new_cons. }
-    rewrite H0.
-    apply in_inv in H. destruct H. rewrite <- H; rewrite e.
-    assert (S n <= first_new (S n) l). apply first_new_nondecreasing. lia.
-    apply IHl. assumption.
- -- (* Case: a <> n *) 
-    apply in_inv in H. destruct H.
-    + rewrite H; rewrite H in n0.
-      assert(first_new n (x::l) = first_new n l). { apply first_new_distinct. assumption. }
-      rewrite H0.
-      assert(decidable (In x l)). { apply (In_decidable Nat.eq_decidable). }
-      destruct H1.
-   ++ apply (IHl n x) in H1. assumption.
-   ++ assert (n <= first_new n l). { apply first_new_nondecreasing. }
-      
-    lia.
-    
-  induction l.
-  - simpl; auto.
-  - intros. assert ({a = n} + {a <> n}). decide equality. destruct H0.
- -- (* Case: a = n *) 
-    rewrite e.
-    assert(first_new n (n::l) = first_new (S n) l). { apply first_new_cons. }
-    rewrite H0.
-    apply in_inv in H. destruct H. rewrite <- H; rewrite e.
-    assert (S n <= first_new (S n) l). apply first_new_nondecreasing. lia.
-    apply IHl. assumption.
- -- (* Case: a <> n *) 
-    apply in_inv in H. destruct H.
-    + rewrite H; rewrite H in n0.
-      assert(first_new n (x::l) = first_new n l). { apply first_new_distinct. assumption. }
-      rewrite H0.
-    Check @first_new_nondecreasing.
- -- (* a = x *)
-    rewrite H. intros.
-    
- -- (* In x l *)
-  assert ({a = n} + {a <> n}). decide equality. destruct H.
-  - assert(first_new n (n::l) = first_new (S n) l). { apply first_new_cons. }
-    rewrite e. rewrite H. Check @first_new_nondecreasing.
-    assert (S n <= first_new (S n) l). { apply first_new_nondecreasing. }
-    lia.
-  - assert(first_new n (a::l) = first_new n l). { apply first_new_distinct. assumption. }
-    
-(* 
-@first_new_nondecreasing
-     : forall (l : list nat) (n : nat),
-       n <= first_new n l
-*)
-    
-    unfold first_new. lia.
-  induction l.
-  - destruct H.
- -- assert(first_new n [n] = first_new (S n) []). { apply first_new_cons. }
-    rewrite e. rewrite H. unfold first_new. lia.
- -- Check @first_new_distinct.
-  apply (@first_new_distinct List.nil a n) in n0 as H.
-    rewrite H. unfold first_new. intuition.
-  - 
-   destruct H.
-  - assert(first_new n (n :: l) = first_new (S n) l). { apply first_new_cons. }
-    rewrite <- H.
-Qed.
-
-
-
-Theorem first_new_is_not_on_list {l n} :
-  ~In (first_new n l) l.
-Proof.
-  generalize dependent n. induction l.
-  - simpl; auto.
-  - intros. apply not_in_cons. split.
- -- assert ({n = a} + {n <> a}). decide equality. destruct H.
---- rewrite <- e.
-    assert(first_new n (n :: l) = first_new (S n) l). { apply first_new_cons. }
-    rewrite H. intuition.
-    
-Lemma first_new_is_new {l a n} :
-  first_new n (a::l) <> a.
-  
-  set (t := (first_new n (a :: l))).
-    apply not_in_cons. split. 
-  -- (* Subcase: t <> a *)
-     assert ({n = a} + {n <> a}). decide equality. destruct H.
-     + (* Sub-subcase: t = first_new n (n :: l) *)
-       assert (t = first_new n (n :: l)).
-       assert (t = first_new n (a :: l)). simpl; auto.
-       rewrite <- e in H. assumption.
-       apply (first_new_cons n l) in H.
-       
-      apply first_new_cons.
-    rewrite <- e in t. 
-  unfold first_new in (first_new n (a :: l)).
-  intros.
 
 Definition fresh_evar_counter (Γ : list Formula) (p : Formula) : nat :=
 first_new 0 (list_evars (p::Γ)%list).
@@ -778,13 +625,13 @@ Inductive deducible : list Formula -> Formula -> Prop :=
 | ND_exists_intro {Γ p t} :
   Γ ⊢ (subst_bvar_inner 0 t p) -> 
   Γ ⊢ Exists p
-| ND_proof_by_contradiction {Γ p} :
-  (Not p) :: Γ ⊢ Falsum ->
-  Γ ⊢ p
 | ND_exists_elim_small {Γ p q c} :
   (subst_bvar_inner 0 c p)::Γ ⊢ q -> 
   c = fresh_evar Γ q ->
   (Exists p)::Γ ⊢ q
+| ND_proof_by_contradiction {Γ p} :
+  (Not p) :: Γ ⊢ Falsum ->
+  Γ ⊢ p
 | ND_prioritize {Γ p q} :
   Γ ⊢ q ->
   In p Γ ->
@@ -829,7 +676,8 @@ Proof.
   apply ND_exists_elim_small in H1.
   apply ND_imp_i2 in H1. 
   apply (@ND_imp_e Γ (Exists p) q ) in H1. 
-  assumption. assumption. assumption.
+  assumption. assumption.
+  assumption.
 Qed.
 
 (**
@@ -962,7 +810,7 @@ Proof.
   intros. simpl; auto.
   assert (In P0 Γ2). { apply subcontext_cons in H; destruct H; assumption. }
   unfold fresh in H0; unfold FreshContext in H0.
-  apply (Forall_forall) with (P := (fun fm : Formula => fresh c fm)) in H1 as H2.
+  apply (List.Forall_forall) with (P := (fun fm : Formula => fresh c fm)) in H1 as H2.
   simpl; auto. simpl; auto.
 Qed.
 
@@ -989,10 +837,40 @@ Proof.
   assert (Γ2 ⊆ a :: Γ2). apply cons_subcontext.
   assert (Γ2 ⊆ Γ1).
   apply (subcontext_trans Γ2 (a :: Γ2) Γ1); assumption; assumption.
-  apply Forall_cons_iff. split.
+  apply List.Forall_cons_iff. split.
   apply IHΓ2 in H2 as IH. apply (fresh_in_head H). assumption.
   apply IHΓ2 in H2 as IH. assumption.
 Qed.
+
+(*
+Definition fresh_evar_counter (Γ : list Formula) (p : Formula) : nat :=
+first_new 0 (list_evars (p::Γ)%list).
+
+Check fresh_evar. Check fresh.
+Theorem lemma_list_evars : forall (Γ1 Γ2 : list Formula),
+  Γ1 ⊆ Γ2 -> incl (list_evars Γ1) (list_evars Γ2).
+Proof. intros.
+*)
+  
+Theorem fresh_econst : forall (Γ1 Γ2 : list Formula) (p : Formula),
+  Γ1 ⊆ Γ2 -> fresh (fresh_evar Γ2 p) Γ1.
+Proof.
+  intros. set (c := (fresh_evar Γ2 p)).
+  assert (fresh c Γ2). { apply fresh_evar_context. }
+  assert (c = c). { reflexivity. }
+  apply (fresh_cons_proper c c H1 _ _ H).
+  assumption.
+Qed.
+
+Axiom renaming_econst : forall (Γ1 Γ2 : list Formula) (p q : Formula),
+  Γ1 ⊆ Γ2 -> 
+  subst_bvar_inner 0 (fresh_evar Γ1 q) p :: Γ1 ⊢ q -> 
+  subst_bvar_inner 0 (fresh_evar Γ2 q) p :: Γ2 ⊢ q.
+
+Axiom renaming_econst2 : forall (Γ1 Γ2 : list Formula) (p : Formula) (c : Term),
+  Γ1 ⊆ Γ2 -> 
+  c = (fresh_evar Γ1 p) -> 
+  c = (fresh_evar Γ2 p).
 
 Lemma subcontext_in_trans {Γ1 Γ2 p} :
   In p Γ1 -> Γ1 ⊆ Γ2 -> In p Γ2.
@@ -1018,22 +896,18 @@ intros Γ₁ Γ₂ ? P Q [] ?. revert Γ₂ H. induction H0; intros.
 + apply (ND_cut (P := P0)); auto.
   apply IHdeducible2. f_equiv. assumption.
 + apply (ND_exists_intro (p := p) (t := t)); auto.
-+ apply ND_proof_by_contradiction. apply IHdeducible. f_equiv. auto.
-
-+ admit. (* apply (ND_unprioritize (p := Exists p) (Γ := Γ₂)).
++ apply subcontext_cons in H1 as H2. destruct H2.
+  apply @renaming_econst2 with (c := c) (p := q) in H3 as H4.
+  apply (ND_unprioritize (p := Exists p) (Γ := Γ₂)).
   apply (ND_exists_elim_small (Γ := Γ₂) (c := c)).
-  apply IHdeducible.
-
-Check @ND_exists_elim_small.
- apply ND_exists_elim_small.
- *)
-+ Check @subcontext_cons.
- apply (@subcontext_cons Γ Γ₂ p) in H1 as H2. apply IHdeducible. destruct H2. assumption.
+  apply IHdeducible. f_equiv. assumption. assumption. assumption. assumption.
++ apply ND_proof_by_contradiction. apply IHdeducible. f_equiv. auto.
++ apply (@subcontext_cons Γ Γ₂ p) in H1 as H2. apply IHdeducible. destruct H2. 
+  assumption.
 + apply IHdeducible. apply (@subcontext_cons Γ Γ₂ p). split.
   apply (@subcontext_in_trans Γ Γ₂).
 assumption. assumption. assumption.
-Admitted.
-(* Qed. *)
+Qed.
 
   
 Theorem weakening : forall (Γ1 Γ2 : list Formula) (P : Formula),
@@ -1447,23 +1321,6 @@ Proof.
   simpl; auto.
   apply ND_imp_i2; apply ND_assume; prove_In.
 Qed.
-
-Theorem exists_modus_ponens_tautology {Γ p q} :
-  Γ ⊢ (Implies (Forall (Implies p q)) (Implies (Exists p) (Exists q))).
-Proof.
-  Assume ((Exists p) :: (Forall (Implies p q)) :: Γ ⊢ (Forall (Implies p q))).
-  Assume ((Exists p) :: (Forall (Implies p q)) :: Γ ⊢ (Exists p)).
-  set (t := fresh_evar ((Exists p) :: (Forall (Implies p q)) :: Γ) q).
-  apply (ND_forall_elim (t := t)) in H. simpl in H.
-  apply (ND_exists_elim (Γ := Exists p :: Forall (Implies p q) :: Γ)  (q := (subst_bvar_inner 0 t q)) (c := t)) in H0 as H1.  
-  apply (ND_imp_e (p := subst_bvar_inner 0 t p) (q := (subst_bvar_inner 0 t q))) in H as H2.
-  apply (ND_exists_intro (Γ := Exists p :: Forall (Implies p q) :: Γ) (t := t) (p := q)) in H2 as H3.
-  apply (@ND_imp_i2 (Forall (Implies p q) :: Γ)) in H3 as H4.
-  apply ND_imp_i2 in H4 as H5. assumption. assumption. assumption.
-  intros.
-  
-  Check ND_exists_elim_small.
-  
 End ImportantTheorems.
 
 Theorem consistency : not (proves Falsum).
